feat(HOL_To_IMP_Minus) tune auto set up of goals and performance

HOL_To_IMP_Minus/Refinements/HOL_To_IMP_Minus_Primitives.thy
@@ -2,13 +2,12 @@
 theory HOL_To_IMP_Minus_Primitives
   imports
     HOL_To_IMP_Tailcalls_Tactics
+    HOL_To_IMP_Minus_Goal_Commands
 begin
-
+term tailcall_to_IMP_Minus
 locale HOL_To_IMP_Minus =
   notes neq0_conv[iff del, symmetric, iff]
 begin
-
-named_theorems func_correct
 
 definition "is_true_nat n \<equiv> n \<noteq> 0"
 
@@ -27,16 +26,16 @@ compile_nat true_nat_def basename true
 declare_compiled_const True
   return_register "true_ret"
   argument_registers
-  compiled "tailcall_to_IMP_Minus true_IMP"
+  compiled "tailcall_to_IMP_Minus true_IMP_tailcall"
 
-lemma true_IMP_func_correct[func_correct]:
-  assumes "(tailcall_to_IMP_Minus true_IMP, s) \<Rightarrow>\<^bsup>t\<^esup> s'"
-  shows "s' ''true_ret'' = true_nat"
-  using assms
-  apply (rule tailcall_to_IMP_Minus_correct_if_correct)
-  apply (subst compiled_const_defs, simp)
-  apply (subst compiled_const_defs, simp)
-  apply (tactic \<open>H.start_run_finish_no_pattern_fun_tac @{thms compiled_const_defs} @{thms func_correct} 
+method preprocess_HOL_To_IMP_Minus_func_correct =
+  (erule tailcall_to_IMP_Minus_correct_if_correct),
+  (subst compiled_const_defs, simp),
+  (subst compiled_const_defs, simp)
+
+HOL_To_IMP_Minus_func_correct true_nat
+  apply preprocess_HOL_To_IMP_Minus_func_correct
+  apply (tactic \<open>H.start_run_finish_no_pattern_fun_tac @{thms compiled_const_defs} @{thms IMP_Minus_func_correct}
     @{thms true_nat_def} @{context} 1\<close>)
   done
 
@@ -46,23 +45,18 @@ lemma true_nat_eq_one[simp]: "true_nat = 1"
 lemma is_true_nat_true_nat[iff]: "is_true_nat true_nat"
   by simp
 
-definition "false_nat \<equiv> 0"
+definition "false_nat \<equiv> (0 :: nat)"
 
 compile_nat false_nat_def basename false
 
 declare_compiled_const False
   return_register "false_ret"
   argument_registers
-  compiled "tailcall_to_IMP_Minus false_IMP"
+  compiled "tailcall_to_IMP_Minus false_IMP_tailcall"
 
-lemma false_IMP_func_correct [func_correct]:
-  assumes "(tailcall_to_IMP_Minus false_IMP, s) \<Rightarrow>\<^bsup>t\<^esup> s'"
-  shows "s' ''false_ret'' = false_nat"
-  using assms
-  apply (rule tailcall_to_IMP_Minus_correct_if_correct)
-  apply (subst compiled_const_defs, simp)
-  apply (subst compiled_const_defs, simp)
-  apply (tactic \<open>H.start_run_finish_no_pattern_fun_tac @{thms compiled_const_defs} @{thms func_correct}
+HOL_To_IMP_Minus_func_correct false_nat
+  apply preprocess_HOL_To_IMP_Minus_func_correct
+  apply (tactic \<open>H.start_run_finish_no_pattern_fun_tac @{thms compiled_const_defs} @{thms IMP_Minus_func_correct}
     @{thms false_nat_def} @{context} 1\<close>)
   done
 
@@ -72,18 +66,13 @@ lemma false_nat_eq_one[simp]: "false_nat = 0"
 lemma is_false_nat_false_nat[iff]: "is_false_nat false_nat"
   unfolding false_nat_def by simp
 
-definition "id_nat x \<equiv> x"
+definition "id_nat x \<equiv> (x :: nat)"
 
 compile_nat id_nat_def basename id
 
-lemma id_IMP_func_correct [func_correct]:
-  assumes "(tailcall_to_IMP_Minus id_IMP, s) \<Rightarrow>\<^bsup>t\<^esup> s'"
-  shows "s' ''id_ret'' = id_nat (s ''id_x'')"
-  using assms
-  apply (rule tailcall_to_IMP_Minus_correct_if_correct)
-  apply (subst compiled_const_defs, simp)
-  apply (subst compiled_const_defs, simp)
-  apply (tactic \<open>H.start_run_finish_no_pattern_fun_tac @{thms compiled_const_defs} @{thms func_correct}
+HOL_To_IMP_Minus_func_correct id_nat
+  apply preprocess_HOL_To_IMP_Minus_func_correct
+  apply (tactic \<open>H.start_run_finish_no_pattern_fun_tac @{thms compiled_const_defs} @{thms IMP_Minus_func_correct}
     @{thms id_nat_def} @{context} 1\<close>)
   done
 
@@ -95,7 +84,7 @@ definition "nat_of_bool b \<equiv> if b then true_nat else false_nat"
 declare_compiled_const nat_of_bool
   return_register "id_ret"
   argument_registers "id_x"
-  compiled "tailcall_to_IMP_Minus id_IMP"
+  compiled "tailcall_to_IMP_Minus id_IMP_tailcall"
 
 lemma nat_of_bool_eq_zero_iff[iff]: "nat_of_bool b = 0 \<longleftrightarrow> \<not>b"
   unfolding nat_of_bool_def by simp
@@ -129,10 +118,8 @@ declare_compiled_const HOL.eq
   argument_registers "eq_x" "eq_y"
   compiled eq_IMP
 
-lemma eq_IMP_func_correct [func_correct]:
-  assumes "(eq_IMP, s) \<Rightarrow>\<^bsup>t\<^esup> s'"
-  shows "s' ''eq_ret'' = eq_nat (s ''eq_x'') (s ''eq_y'')"
-  using assms unfolding eq_IMP_def eq_nat_def nat_of_bool_def by auto
+HOL_To_IMP_Minus_func_correct eq_nat
+  unfolding eq_IMP_def eq_nat_def nat_of_bool_def by auto
 
 lemma eq_nat_eq_nat_of_bool_eq[simp]: "eq_nat n m = nat_of_bool (n = m)"
   unfolding eq_nat_def by simp
@@ -144,16 +131,11 @@ compile_nat not_nat_def basename not
 declare_compiled_const HOL.Not
   return_register "not_ret"
   argument_registers "not_n"
-  compiled "tailcall_to_IMP_Minus not_IMP"
+  compiled "tailcall_to_IMP_Minus not_IMP_tailcall"
 
-lemma not_IMP_func_correct [func_correct]:
-  assumes "(tailcall_to_IMP_Minus not_IMP, s) \<Rightarrow>\<^bsup>t\<^esup> s'"
-  shows "s' ''not_ret'' = not_nat (s ''not_n'')"
-  using assms                                 
-  apply (rule tailcall_to_IMP_Minus_correct_if_correct)
-  apply (subst compiled_const_defs, simp)
-  apply (subst compiled_const_defs, simp)
-  apply (tactic \<open>H.start_run_finish_no_pattern_fun_tac @{thms compiled_const_defs} @{thms func_correct} 
+HOL_To_IMP_Minus_func_correct not_nat
+  apply preprocess_HOL_To_IMP_Minus_func_correct
+  apply (tactic \<open>H.start_run_finish_no_pattern_fun_tac @{thms compiled_const_defs} @{thms IMP_Minus_func_correct}
     @{thms not_nat_def} @{context} 1\<close>)
   done
 
@@ -161,23 +143,18 @@ lemma not_nat_eq_nat_of_bool_eq_false[simp]: "not_nat n = nat_of_bool (n = false
   unfolding not_nat_def by simp
 
 definition max_nat :: "nat \<Rightarrow> nat \<Rightarrow> nat" where
-  "max_nat x y \<equiv> if x - y \<noteq> 0 then x else y"  
+  "max_nat x y \<equiv> if x - y \<noteq> 0 then x else y"
 
 compile_nat max_nat_def basename max
 
 declare_compiled_const max
   return_register "max_ret"
   argument_registers "max_x" "max_y"
-  compiled "tailcall_to_IMP_Minus max_IMP"
+  compiled "tailcall_to_IMP_Minus max_IMP_tailcall"
 
-lemma max_IMP_func_correct[func_correct]:
-  assumes "(tailcall_to_IMP_Minus max_IMP, s) \<Rightarrow>\<^bsup>t\<^esup> s'"
-  shows "s' ''max_ret'' = max_nat (s ''max_x'') (s ''max_y'')"
-  using assms                                 
-  apply (rule tailcall_to_IMP_Minus_correct_if_correct)
-  apply (subst compiled_const_defs, simp)
-  apply (subst compiled_const_defs, simp)
-  apply (tactic \<open>H.start_run_finish_no_pattern_fun_tac @{thms compiled_const_defs} @{thms func_correct} 
+HOL_To_IMP_Minus_func_correct max_nat
+  apply preprocess_HOL_To_IMP_Minus_func_correct
+  apply (tactic \<open>H.start_run_finish_no_pattern_fun_tac @{thms compiled_const_defs} @{thms IMP_Minus_func_correct}
     @{thms max_nat_def} @{context} 1\<close>)
   done
 
@@ -192,16 +169,11 @@ compile_nat min_nat_def basename min
 declare_compiled_const min
   return_register "min_ret"
   argument_registers "min_x" "min_y"
-  compiled "tailcall_to_IMP_Minus min_IMP"
+  compiled "tailcall_to_IMP_Minus min_IMP_tailcall"
 
-lemma min_IMP_func_correct[func_correct]:
-  assumes "(tailcall_to_IMP_Minus min_IMP, s) \<Rightarrow>\<^bsup>t\<^esup> s'"
-  shows "s' ''min_ret'' = min_nat (s ''min_x'') (s ''min_y'')"
-  using assms                                 
-  apply (rule tailcall_to_IMP_Minus_correct_if_correct)
-  apply (subst compiled_const_defs, simp)
-  apply (subst compiled_const_defs, simp)
-  apply (tactic \<open>H.start_run_finish_no_pattern_fun_tac @{thms compiled_const_defs} @{thms func_correct} 
+HOL_To_IMP_Minus_func_correct min_nat
+  apply preprocess_HOL_To_IMP_Minus_func_correct
+  apply (tactic \<open>H.start_run_finish_no_pattern_fun_tac @{thms compiled_const_defs} @{thms IMP_Minus_func_correct}
     @{thms min_nat_def} @{context} 1\<close>)
   done
 
@@ -209,22 +181,17 @@ lemma min_nat_eq[simp]: "min_nat x y = min x y"
   unfolding min_nat_def by simp
 
 definition "and_nat (x :: nat) y \<equiv> min (min x y) true_nat"
-  
+
 compile_nat and_nat_def basename "and"
 
 declare_compiled_const conj
   return_register "and_ret"
   argument_registers "and_x" "and_y"
-  compiled "tailcall_to_IMP_Minus and_IMP"
+  compiled "tailcall_to_IMP_Minus and_IMP_tailcall"
 
-lemma and_nat_IMP_func_correct[func_correct]:
-  assumes "(tailcall_to_IMP_Minus and_IMP, s) \<Rightarrow>\<^bsup>t\<^esup> s'"
-  shows "s' ''and_ret'' = and_nat (s ''and_x'') (s ''and_y'')"
-  using assms                                 
-  apply (rule tailcall_to_IMP_Minus_correct_if_correct)
-  apply (subst compiled_const_defs, simp)
-  apply (subst compiled_const_defs, simp)
-  apply (tactic \<open>H.start_run_finish_no_pattern_fun_tac @{thms compiled_const_defs} @{thms func_correct} 
+HOL_To_IMP_Minus_func_correct and_nat
+  apply preprocess_HOL_To_IMP_Minus_func_correct
+  apply (tactic \<open>H.start_run_finish_no_pattern_fun_tac @{thms compiled_const_defs} @{thms IMP_Minus_func_correct}
     @{thms and_nat_def} @{context} 1\<close>)
   done
 
@@ -238,16 +205,11 @@ compile_nat or_nat_def basename "or"
 declare_compiled_const disj
   return_register "or_ret"
   argument_registers "or_x" "or_y"
-  compiled "tailcall_to_IMP_Minus or_IMP"
+  compiled "tailcall_to_IMP_Minus or_IMP_tailcall"
 
-lemma or_nat_IMP_func_correct[func_correct]:
-  assumes "(tailcall_to_IMP_Minus or_IMP, s) \<Rightarrow>\<^bsup>t\<^esup> s'"
-  shows "s' ''or_ret'' = or_nat (s ''or_x'') (s ''or_y'')"
-  using assms                                 
-  apply (rule tailcall_to_IMP_Minus_correct_if_correct)
-  apply (subst compiled_const_defs, simp)
-  apply (subst compiled_const_defs, simp)
-  apply (tactic \<open>H.start_run_finish_no_pattern_fun_tac @{thms compiled_const_defs} @{thms func_correct} 
+HOL_To_IMP_Minus_func_correct or_nat
+  apply preprocess_HOL_To_IMP_Minus_func_correct
+  apply (tactic \<open>H.start_run_finish_no_pattern_fun_tac @{thms compiled_const_defs} @{thms IMP_Minus_func_correct}
     @{thms or_nat_def} @{context} 1\<close>)
   done
 
@@ -261,16 +223,11 @@ compile_nat le_nat_def basename le
 declare_compiled_const "ord_class.less_eq"
   return_register "le_ret"
   argument_registers "le_x" "le_y"
-  compiled "tailcall_to_IMP_Minus le_IMP"
+  compiled "tailcall_to_IMP_Minus le_IMP_tailcall"
 
-lemma le_nat_IMP_func_correct[func_correct]:
-  assumes "(tailcall_to_IMP_Minus le_IMP, s) \<Rightarrow>\<^bsup>t\<^esup> s'"
-  shows "s' ''le_ret'' = le_nat (s ''le_x'') (s ''le_y'')"
-  using assms                                 
-  apply (rule tailcall_to_IMP_Minus_correct_if_correct)
-  apply (subst compiled_const_defs, simp)
-  apply (subst compiled_const_defs, simp)
-  apply (tactic \<open>H.start_run_finish_no_pattern_fun_tac @{thms compiled_const_defs} @{thms func_correct} 
+HOL_To_IMP_Minus_func_correct le_nat
+  apply preprocess_HOL_To_IMP_Minus_func_correct
+  apply (tactic \<open>H.start_run_finish_no_pattern_fun_tac @{thms compiled_const_defs} @{thms IMP_Minus_func_correct}
     @{thms le_nat_def} @{context} 1\<close>)
   done
 
@@ -284,16 +241,11 @@ compile_nat lt_nat_def basename lt
 declare_compiled_const "ord_class.less"
   return_register "lt_ret"
   argument_registers "lt_x" "lt_y"
-  compiled "tailcall_to_IMP_Minus lt_IMP"
+  compiled "tailcall_to_IMP_Minus lt_IMP_tailcall"
 
-lemma lt_nat_IMP_func_correct[func_correct]:
-  assumes "(tailcall_to_IMP_Minus lt_IMP, s) \<Rightarrow>\<^bsup>t\<^esup> s'"
-  shows "s' ''lt_ret'' = lt_nat (s ''lt_x'') (s ''lt_y'')"
-  using assms                                 
-  apply (rule tailcall_to_IMP_Minus_correct_if_correct)
-  apply (subst compiled_const_defs, simp)
-  apply (subst compiled_const_defs, simp)
-  apply (tactic \<open>H.start_run_finish_no_pattern_fun_tac @{thms compiled_const_defs} @{thms func_correct} 
+HOL_To_IMP_Minus_func_correct lt_nat
+  apply preprocess_HOL_To_IMP_Minus_func_correct
+  apply (tactic \<open>H.start_run_finish_no_pattern_fun_tac @{thms compiled_const_defs} @{thms IMP_Minus_func_correct}
     @{thms lt_nat_def} @{context} 1\<close>)
   done
 
