HOL_To_IMP_Minus/Refinements/HOL_To_IMP_Minus_Arithmetics.thy
@@ -11,33 +11,26 @@ begin
 definition [compiled_const_defs add]: "suc_IMP \<equiv> Com.Assign ''suc_ret'' (V ''suc_x'' \<oplus> N 1)"
 
 declare_compiled_const Suc
-  return_register "suc_ret"                                                     
+  return_register "suc_ret"
   argument_registers "suc_x"
   compiled suc_IMP
 
-lemma suc_IMP_func_correct [func_correct]:
-  assumes "(suc_IMP, s) \<Rightarrow>\<^bsup>t\<^esup> s'"
-  shows "s' ''suc_ret'' = Suc (s ''suc_x'')"
-  using assms unfolding suc_IMP_def by auto
+HOL_To_IMP_Minus_func_correct Suc
+  unfolding suc_IMP_def by auto
 
 fun mul_acc_nat :: "nat \<Rightarrow> nat \<Rightarrow> nat \<Rightarrow> nat" where
 "mul_acc_nat 0 _ z = z" |
 "mul_acc_nat (Suc x) y z = mul_acc_nat x y (y + z)"
 declare mul_acc_nat.simps[simp del]
-                        
+
 case_of_simps mul_acc_nat_eq[simplified Nitpick.case_nat_unfold] : mul_acc_nat.simps
 compile_nat mul_acc_nat_eq basename mul_acc
 
-lemma mul_acc_nat_IMP_func_correct[func_correct]:
-  assumes "(tailcall_to_IMP_Minus mul_acc_IMP, s) \<Rightarrow>\<^bsup>t\<^esup> s'"
-  shows "s' ''mul_acc_ret'' = mul_acc_nat (s ''mul_acc_x1a'') (s ''mul_acc_x2a'') (s ''mul_acc_x3ba'')"
-  using assms                                 
-  apply (rule tailcall_to_IMP_Minus_correct_if_correct)
-  apply (subst compiled_const_defs, simp)
-  apply (subst compiled_const_defs, simp)
+HOL_To_IMP_Minus_func_correct mul_acc_nat
+  apply preprocess_HOL_To_IMP_Minus_func_correct
   subgoal for t s'
   apply (induction "(s ''mul_acc_x1a'')" "(s ''mul_acc_x2a'')" "(s ''mul_acc_x3ba'')" arbitrary: s t rule: mul_acc_nat.induct)
-  apply (tactic \<open>H.start_run_finish_pattern_fun_tac @{thms compiled_const_defs} @{thms func_correct} 
+  apply (tactic \<open>H.start_run_finish_pattern_fun_tac @{thms compiled_const_defs} @{thms IMP_Minus_func_correct}
     @{thms mul_acc_nat.simps} @{context} 1\<close>)+
   done
   done
@@ -45,25 +38,20 @@ lemma mul_acc_nat_IMP_func_correct[func_correct]:
 lemma mul_acc_nat_eq_mul_add[simp]: "mul_acc_nat x y z = x * y + z"
   by (induction x y z arbitrary: z rule: mul_acc_nat.induct)
   (auto simp: mul_acc_nat.simps mult_eq_if)
-  
+
 definition mul_nat :: "nat \<Rightarrow> nat \<Rightarrow> nat" where
   "mul_nat x y = mul_acc_nat x y 0"
-  
+
 compile_nat mul_nat_def basename mul
 
 declare_compiled_const "times"
   return_register "mul_ret"
   argument_registers "mul_x" "mul_y"
-  compiled "tailcall_to_IMP_Minus mul_IMP"
+  compiled "tailcall_to_IMP_Minus mul_IMP_tailcall"
 
-lemma mul_nat_IMP_func_correct[func_correct]:
-  assumes "(tailcall_to_IMP_Minus mul_IMP, s) \<Rightarrow>\<^bsup>t\<^esup> s'"
-  shows "s' ''mul_ret'' = mul_nat (s ''mul_x'') (s ''mul_y'')"
-  using assms                                 
-  apply (rule tailcall_to_IMP_Minus_correct_if_correct)
-  apply (subst compiled_const_defs, simp)
-  apply (subst compiled_const_defs, simp)
-  apply (tactic \<open>H.start_run_finish_no_pattern_fun_tac @{thms compiled_const_defs} @{thms func_correct} 
+HOL_To_IMP_Minus_func_correct mul_nat
+  apply preprocess_HOL_To_IMP_Minus_func_correct
+  apply (tactic \<open>H.start_run_finish_no_pattern_fun_tac @{thms compiled_const_defs} @{thms IMP_Minus_func_correct}
     @{thms mul_nat_def} @{context} 1\<close>)
   done
 
@@ -76,16 +64,11 @@ declare div_acc_nat.simps[simp del]
 
 compile_nat div_acc_nat.simps basename div_acc
 
-lemma div_acc_nat_IMP_func_correct[func_correct]:
-  assumes "(tailcall_to_IMP_Minus div_acc_IMP, s) \<Rightarrow>\<^bsup>t\<^esup> s'"
-  shows "s' ''div_acc_ret'' = div_acc_nat (s ''div_acc_x'') (s ''div_acc_y'') (s ''div_acc_z'')"
-  using assms                                 
-  apply (rule tailcall_to_IMP_Minus_correct_if_correct)
-  apply (subst compiled_const_defs, simp)
-  apply (subst compiled_const_defs, simp)
+HOL_To_IMP_Minus_func_correct div_acc_nat
+  apply preprocess_HOL_To_IMP_Minus_func_correct
   subgoal for t s'
   apply (induction "(s ''div_acc_x'')" "(s ''div_acc_y'')" "(s ''div_acc_z'')" arbitrary: s t rule: div_acc_nat.induct)
-  apply (tactic \<open>H.start_run_finish_no_pattern_fun_tac @{thms compiled_const_defs} @{thms func_correct}
+  apply (tactic \<open>H.start_run_finish_no_pattern_fun_tac @{thms compiled_const_defs} @{thms IMP_Minus_func_correct}
     @{thms div_acc_nat.simps} @{context} 1\<close>)
   done
   done
@@ -101,16 +84,11 @@ compile_nat div_nat_def basename div
 declare_compiled_const "divide"
   return_register "div_ret"
   argument_registers "div_x" "div_y"
-  compiled "tailcall_to_IMP_Minus div_IMP"
+  compiled "tailcall_to_IMP_Minus div_IMP_tailcall"
 
-lemma div_nat_IMP_func_correct[func_correct]:
-  assumes "(tailcall_to_IMP_Minus div_IMP, s) \<Rightarrow>\<^bsup>t\<^esup> s'"
-  shows "s' ''div_ret'' = div_nat (s ''div_x'') (s ''div_y'')"
-  using assms                                 
-  apply (rule tailcall_to_IMP_Minus_correct_if_correct)
-  apply (subst compiled_const_defs, simp)
-  apply (subst compiled_const_defs, simp)
-  apply (tactic \<open>H.start_run_finish_no_pattern_fun_tac @{thms compiled_const_defs} @{thms func_correct}
+HOL_To_IMP_Minus_func_correct div_nat
+  apply preprocess_HOL_To_IMP_Minus_func_correct
+  apply (tactic \<open>H.start_run_finish_no_pattern_fun_tac @{thms compiled_const_defs} @{thms IMP_Minus_func_correct}
     @{thms div_nat_def} @{context} 1\<close>)
   done
 
@@ -119,17 +97,12 @@ lemma div_nat_eq_div[simp]: "div_nat x y = x div y"
 
 definition square_nat :: "nat \<Rightarrow> nat" where
   "square_nat x \<equiv> mul_nat x x"
-  
+
 compile_nat square_nat_def basename square
 
-lemma square_nat_IMP_func_correct[func_correct]:
-  assumes "(tailcall_to_IMP_Minus square_IMP, s) \<Rightarrow>\<^bsup>t\<^esup> s'"
-  shows "s' ''square_ret'' = square_nat (s ''square_x'')"
-  using assms                                 
-  apply (rule tailcall_to_IMP_Minus_correct_if_correct)
-  apply (subst compiled_const_defs, simp)
-  apply (subst compiled_const_defs, simp)
-  apply (tactic \<open>H.start_run_finish_no_pattern_fun_tac @{thms compiled_const_defs} @{thms func_correct} 
+HOL_To_IMP_Minus_func_correct square_nat
+  apply preprocess_HOL_To_IMP_Minus_func_correct
+  apply (tactic \<open>H.start_run_finish_no_pattern_fun_tac @{thms compiled_const_defs} @{thms IMP_Minus_func_correct}
      @{thms square_nat_def} @{context} 1\<close>)
   done
 
@@ -139,12 +112,12 @@ lemma square_nat_eq_square[simp]: "square_nat x = x\<^sup>2"
 (*takes lower and upper bound for root*)
 function sqrt_aux_nat :: "nat \<Rightarrow> nat \<Rightarrow> nat \<Rightarrow> nat" where
   "sqrt_aux_nat x L R = (if Suc L < R
-    then 
+    then
       let M = (L + R) div 2
-      in 
+      in
         if square_nat M \<le> x
-        then sqrt_aux_nat x M R 
-        else sqrt_aux_nat x L M 
+        then sqrt_aux_nat x M R
+        else sqrt_aux_nat x L M
     else L)"
   by auto
 termination by (relation "Wellfounded.measure (\<lambda>(_, L, R). R - L)") auto
@@ -152,16 +125,11 @@ declare sqrt_aux_nat.simps[simp del]
 
 compile_nat sqrt_aux_nat.simps basename sqrt_aux
 
-lemma sqrt_aux_IMP_func_correct[func_correct]:
-  assumes "(tailcall_to_IMP_Minus sqrt_aux_IMP, s) \<Rightarrow>\<^bsup>t\<^esup> s'"
-  shows "s' ''sqrt_aux_ret'' = sqrt_aux_nat (s ''sqrt_aux_x'') (s ''sqrt_aux_L'') (s ''sqrt_aux_R'')"
-  using assms                                 
-  apply (rule tailcall_to_IMP_Minus_correct_if_correct)
-  apply (subst compiled_const_defs, simp)
-  apply (subst compiled_const_defs, simp)
+HOL_To_IMP_Minus_func_correct sqrt_aux_nat
+  apply preprocess_HOL_To_IMP_Minus_func_correct
   subgoal for t s'
   apply (induction "s ''sqrt_aux_x''" "s ''sqrt_aux_L''" "s ''sqrt_aux_R''" arbitrary: s t rule: sqrt_aux_nat.induct)
-  apply (tactic \<open>H.start_run_finish_no_pattern_fun_tac @{thms compiled_const_defs} @{thms func_correct} 
+  apply (tactic \<open>H.start_run_finish_no_pattern_fun_tac @{thms compiled_const_defs} @{thms IMP_Minus_func_correct}
      @{thms sqrt_aux_nat.simps} @{context} 1\<close>)
   done
   done
@@ -172,7 +140,7 @@ lemma square_sqrt_aux_nat_le:
   using assms
   by (induction x L R rule: sqrt_aux_nat.induct)
   (auto simp: sqrt_aux_nat.simps Let_def)
-  
+
 lemma lt_square_Suc_sqrt_aux_nat:
   assumes "L\<^sup>2 \<le> x" "x < R\<^sup>2"
   shows "x < (Suc (sqrt_aux_nat x L R))\<^sup>2"
@@ -185,14 +153,9 @@ definition sqrt_nat :: "nat \<Rightarrow> nat" where
 
 compile_nat sqrt_nat_def basename sqrt
 
-lemma sqrt_IMP_func_correct[func_correct]:
-  assumes "(tailcall_to_IMP_Minus sqrt_IMP, s) \<Rightarrow>\<^bsup>t\<^esup> s'"
-  shows "s' ''sqrt_ret'' = sqrt_nat (s ''sqrt_x'')"
-  using assms                                 
-  apply (rule tailcall_to_IMP_Minus_correct_if_correct)
-  apply (subst compiled_const_defs, simp)
-  apply (subst compiled_const_defs, simp)
-  apply (tactic \<open>H.start_run_finish_no_pattern_fun_tac @{thms compiled_const_defs} @{thms func_correct} 
+HOL_To_IMP_Minus_func_correct sqrt_nat
+  apply preprocess_HOL_To_IMP_Minus_func_correct
+  apply (tactic \<open>H.start_run_finish_no_pattern_fun_tac @{thms compiled_const_defs} @{thms IMP_Minus_func_correct}
      @{thms sqrt_nat_def} @{context} 1\<close>)
   done
 
