HOL_To_IMP_Minus/Refinements/HOL_To_IMP_Minus_Datatypes.thy
@@ -10,14 +10,9 @@ begin
 
 compile_nat triangle_def basename triangle
 
-lemma triangle_IMP_func_correct [func_correct]:
-  assumes "(tailcall_to_IMP_Minus triangle_IMP, s) \<Rightarrow>\<^bsup>t\<^esup> s'"
-  shows "s' ''triangle_ret'' = triangle (s ''triangle_n'')"
-  using assms
-  apply (rule tailcall_to_IMP_Minus_correct_if_correct)
-  apply (subst compiled_const_defs, simp)
-  apply (subst compiled_const_defs, simp)
-  apply (tactic \<open>H.start_run_finish_no_pattern_fun_tac @{thms compiled_const_defs} @{thms func_correct} 
+HOL_To_IMP_Minus_func_correct triangle
+  apply preprocess_HOL_To_IMP_Minus_func_correct
+  apply (tactic \<open>H.start_run_finish_no_pattern_fun_tac @{thms compiled_const_defs} @{thms IMP_Minus_func_correct}
      @{thms triangle_def} @{context} 1\<close>)
   done
 
