HOL_To_IMP_Minus/Refinements/HOL_To_IMP_Minus_Fun_Pattern_Setup.thy
@@ -25,20 +25,15 @@ fun add_nat_pat :: "nat \<Rightarrow> nat \<Rightarrow> nat \<Rightarrow> nat" w
 "add_nat_pat 0 (Suc y) z = add_nat_pat 0 y (z + 1)" |
 "add_nat_pat (Suc x) y z = add_nat_pat x y (z + 1)"
 declare add_nat_pat.simps[simp del]
-                        
+
 case_of_simps add_nat_pat_eq[simplified Nitpick.case_nat_unfold] : add_nat_pat.simps
 compile_nat add_nat_pat_eq basename add_pat
 
-lemma add_nat_pat_IMP_func_correct:
-  assumes "(tailcall_to_IMP_Minus add_pat_IMP, s) \<Rightarrow>\<^bsup>t\<^esup> s'"
-  shows "s' ''add_pat_ret'' = add_nat_pat (s ''add_pat_x1a'') (s ''add_pat_x2a'') (s ''add_pat_x3ba'')"
-  using assms                                 
-  apply (rule tailcall_to_IMP_Minus_correct_if_correct)
-  apply (subst compiled_const_defs, simp)
-  apply (subst compiled_const_defs, simp)
+HOL_To_IMP_Minus_func_correct add_nat_pat
+  apply preprocess_HOL_To_IMP_Minus_func_correct
   subgoal for t s'
   apply (induction "(s ''add_pat_x1a'')" "(s ''add_pat_x2a'')" "(s ''add_pat_x3ba'')" arbitrary: s t rule: add_nat_pat.induct)
-  apply (tactic \<open>H.start_run_finish_pattern_fun_tac @{thms compiled_const_defs} @{thms func_correct} 
+  apply (tactic \<open>H.start_run_finish_pattern_fun_tac @{thms compiled_const_defs} @{thms IMP_Minus_func_correct}
     @{thms add_nat_pat.simps} @{context} 1\<close>)+
   done
   done
